WIP stack object

theories/case_studies/macros/checkra.v
@@ -8,7 +8,8 @@ Section Checkra.
   .
 
 
-  Definition checkra_instrs (r r1 r2 : RegName) : list Word.
+  Definition checkra_instrs (r r1 r2 : RegName) : list Word :=
+    encodeInstrsW [ Mov r1 0%Z; Mov r2 0%Z ].
   (* TODO: it's actually quite annoying to check...
      In CHERIoT, I would do something like:
      ```
@@ -19,7 +20,6 @@ Section Checkra.
      Maybe I should have another instruction in the machine
      for checking this easily?
    *)
-  Admitted.
 
 
 End Checkra.
@@ -30,5 +30,35 @@ Section Checkra_spec.
       {ceriseg: ceriseG Σ}
       {MP: MachineParameters}
   .
+
+  Lemma checkra_spec
+    (rsrc r1 r2 : RegName)
+    (pc_p : Perm) (pc_g : Locality) (pc_b pc_e pc_a : Addr)
+    (wsrc w1 w2 : Word)
+    (φ : language.val cap_lang → iPropI Σ) :
+
+    let checkra_ := (checkra_instrs rsrc r1 r2) in
+    let a_last := (pc_a ^+ length checkra_)%a in
+    executeAllowed pc_p = true →
+    SubBounds pc_b pc_e pc_a a_last →
+
+    ▷ PC ↦ᵣ WCap pc_p pc_g pc_b pc_e pc_a
+    ∗ ▷ rsrc ↦ᵣ wsrc
+    ∗ ▷ r1 ↦ᵣ w1
+    ∗ ▷ r2 ↦ᵣ w2
+    ∗ ▷ codefrag pc_a checkra_
+    ∗ ▷ ( (∃ p g b e a,
+          ⌜ readAllowed p = true ∧ wsrc = WCap p g b e a⌝
+          ∗ PC ↦ᵣ WCap pc_p pc_g pc_b pc_e a_last
+          ∗ rsrc ↦ᵣ WCap p g b e a
+          ∗ r1 ↦ᵣ WInt 0%Z
+          ∗ r2 ↦ᵣ WInt 0%Z
+          ∗ codefrag pc_a checkra_ )
+            -∗ WP Seq (Instr Executable) {{ φ }}
+        )
+    ∗ ▷ φ FailedV
+    ⊢ WP Seq (Instr Executable) {{ φ }}.
+  Proof.
+  Admitted.
 
 End Checkra_spec.
