theories/case_studies/stack_object/stack_object_spec_closure.v
@@ -1,0 +1,820 @@
+From iris.proofmode Require Import proofmode.
+From cap_machine Require Import region_invariants_allocation region_invariants_revocation interp_weakening monotone.
+From cap_machine Require Import rules logrel logrel_extra monotone proofmode register_tactics.
+From cap_machine Require Import fetch_spec assert_spec checkints checkra.
+From cap_machine Require Import
+  switcher interp_switcher_call switcher_spec_call switcher_spec_return.
+From cap_machine Require Import stack_object.
+From cap_machine Require Import proofmode.
+
+Section SO.
+  Context
+    {Σ:gFunctors}
+    {ceriseg:ceriseG Σ} {sealsg: sealStoreG Σ}
+    {Cname : CmptNameG}
+    {stsg : STSG Addr region_type Σ} {heapg : heapGS Σ}
+    {nainv: logrel_na_invs Σ}
+    {cstackg : CSTACKG Σ}
+    `{MP: MachineParameters}
+    {swlayout : switcherLayout}
+  .
+
+  Context {C : CmptName}.
+
+  Implicit Types W : WORLD.
+  Implicit Types C : CmptName.
+  Notation V := (WORLD -n> (leibnizO CmptName) -n> (leibnizO Word) -n> iPropO Σ).
+
+  Lemma stack_object_f_spec
+
+    (pc_b pc_e pc_a : Addr)
+    (cgp_b cgp_e : Addr)
+
+    (b_so_exp_tbl e_so_exp_tbl : Addr)
+    (g_so_exp_tbl : Locality)
+
+    (b_assert e_assert : Addr) (a_flag : Addr)
+    (C_f : Sealable)
+
+    (W : WORLD)
+
+    (Nassert Nswitcher Nso SON : namespace)
+
+    :
+
+    let imports :=
+     so_main_imports
+       b_switcher e_switcher a_switcher_call ot_switcher b_assert e_assert C_f
+    in
+
+    Nswitcher ## Nassert ->
+    Nswitcher ## Nso ->
+    Nassert ## Nso ->
+    (b_so_exp_tbl <= b_so_exp_tbl ^+ 2 < e_so_exp_tbl)%a ->
+    SubBounds pc_b pc_e pc_a (pc_a ^+ length so_main_code)%a ->
+    (pc_b + length imports)%a = Some pc_a ->
+    (cgp_b + length so_main_data)%a = Some cgp_e ->
+
+    na_inv logrel_nais Nassert (assert_inv b_assert e_assert a_flag)
+    ∗ na_inv logrel_nais Nswitcher switcher_inv
+    ∗ na_inv logrel_nais Nso
+        ([[ pc_b , pc_a ]] ↦ₐ [[ imports ]] ∗ codefrag pc_a so_main_code)
+    ∗ inv (export_table_PCCN SON) (b_so_exp_tbl ↦ₐ WCap RX Global pc_b pc_e pc_b)
+    ∗ inv (export_table_CGPN SON) ((b_so_exp_tbl ^+ 1)%a ↦ₐ WCap RW Global cgp_b cgp_e cgp_b)
+    ∗ inv (export_table_entryN SON (b_so_exp_tbl ^+ 2)%a)
+        ((b_so_exp_tbl ^+ 2)%a ↦ₐ WInt (encode_entry_point 1 (length (imports ++ SO_main_code_run))))
+    ∗ WSealed ot_switcher (SCap RO g_so_exp_tbl b_so_exp_tbl e_so_exp_tbl (b_so_exp_tbl ^+ 2)%a)
+        ↦□ₑ 1
+    ∗ seal_pred ot_switcher ot_switcher_propC
+      -∗
+    ot_switcher_prop W C (WCap RO g_so_exp_tbl b_so_exp_tbl e_so_exp_tbl (b_so_exp_tbl ^+ 2)%a).
+  Proof.
+    intros imports.
+    iIntros (Hswitcher_assert HNswitcher_so HNassert_so
+               Hso_exp_tbl_size Hso_size_code Hso_imports Hcgp_size)
+      "(#Hassert & #Hswitcher
+      & #Hso_code
+      & #Hso_exp_PCC
+      & #Hso_exp_CGP
+      & #Hso_exp_awkward
+      & #Hentry_SO & #Hot_switcher)".
+    iExists g_so_exp_tbl, b_so_exp_tbl, e_so_exp_tbl, (b_so_exp_tbl ^+ 2)%a,
+    pc_b, pc_e, cgp_b, cgp_e, 1, _, SON.
+    iFrame "#".
+    iSplit; first done.
+    iSplit; first solve_addr.
+    iSplit; first (iPureIntro; solve_addr).
+    iSplit; first (iPureIntro; solve_addr).
+    iSplit; first (iPureIntro; lia).
+    iIntros "!> %W0 %Hpriv_W_W0 !> %cstk %Ws %Cs %rmap %csp_b' %csp_e".
+    iIntros "(HK & %Hframe_match & Hregister_state & Hrmap & Hr_C & Hsts_C & %Hsync_csp & Hcstk & Hna)".
+    iDestruct "Hregister_state" as
+      "(%Hrmap_init & %HPC & %Hcgp & %Hcra & %Hcsp & #Hinterp_W0_csp & Hinterp_rmap & Hzeroed_rmap)".
+    rewrite /interp_conf.
+    rewrite /registers_pointsto.
+
+    iDestruct (big_sepM_delete _ _ PC with "Hrmap") as "[HPC Hrmap]"; first by simplify_map_eq.
+    iDestruct (big_sepM_delete _ _ cgp with "Hrmap") as "[Hcgp Hrmap]"; first by simplify_map_eq.
+    iDestruct (big_sepM_delete _ _ csp with "Hrmap") as "[Hcsp Hrmap]"; first by simplify_map_eq.
+    iDestruct (big_sepM_delete _ _ cra with "Hrmap") as "[Hcra Hrmap]"; first by simplify_map_eq.
+
+    iMod (na_inv_acc with "Hso_code Hna")
+      as "(( >Himports_main & >Hcode_main) & Hna & Hso_code_close)"; auto.
+    codefrag_facts "Hcode_main" ; rename H into Hpc_contiguous; clear H0.
+
+    (* --- Extract registers ca0  --- *)
+    assert ( is_Some (rmap !! ct0) ) as [wct0 Hwct0].
+    { apply Hrmap_init; rewrite Hrmap_dom ; done. }
+    iDestruct (big_sepM_delete _ _ ct0 with "Hrmap") as "[Hct0 Hrmap]"; first by simplify_map_eq.
+    assert ( is_Some (rmap !! cs0) ) as [wcs0 Hwcs0].
+    { apply Hrmap_init; rewrite Hrmap_dom ; done. }
+    iDestruct (big_sepM_delete _ _ cs0 with "Hrmap") as "[Hcs0 Hrmap]"; first by simplify_map_eq.
+    assert ( is_Some (rmap !! cs1) ) as [wcs1 Hwcs1].
+    { apply Hrmap_init; rewrite Hrmap_dom ; done. }
+    iDestruct (big_sepM_delete _ _ cs1 with "Hrmap") as "[Hcs1 Hrmap]"; first by simplify_map_eq.
+    assert ( is_Some (rmap !! ct1) ) as [wct1 Hwct1].
+    { apply Hrmap_init; rewrite Hrmap_dom ; done. }
+    iDestruct (big_sepM_delete _ _ ct1 with "Hrmap") as "[Hct1 Hrmap]"; first by simplify_map_eq.
+    assert ( is_Some (rmap !! ct2) ) as [wct2 Hwct2].
+    { apply Hrmap_init; rewrite Hrmap_dom ; done. }
+    iDestruct (big_sepM_delete _ _ ct2 with "Hrmap") as "[Hct2 Hrmap]"; first by simplify_map_eq.
+    assert ( is_Some (rmap !! ct3) ) as [wct3 Hwct3].
+    { apply Hrmap_init; rewrite Hrmap_dom ; done. }
+    iDestruct (big_sepM_delete _ _ ct3 with "Hrmap") as "[Hct3 Hrmap]"; first by simplify_map_eq.
+    assert ( is_Some (rmap !! ca0) ) as [wca0 Hwca0].
+    { apply Hrmap_init; rewrite Hrmap_dom ; done. }
+    iDestruct (big_sepM_delete _ _ ca0 with "Hrmap") as "[Hca0 Hrmap]"; first by simplify_map_eq.
+    assert ( is_Some (rmap !! ca1) ) as [wca1 Hwca1].
+    { apply Hrmap_init; rewrite Hrmap_dom ; done. }
+    iDestruct (big_sepM_delete _ _ ca1 with "Hrmap") as "[Hca1 Hrmap]"; first by simplify_map_eq.
+
+    (* Extract the imports *)
+    iDestruct (region_pointsto_cons with "Himports_main") as "[Himport_switcher Himports_main]".
+    { transitivity (Some (pc_b ^+ 1)%a); auto; solve_addr. }
+    { solve_addr. }
+    iDestruct (region_pointsto_cons with "Himports_main") as "[Himport_assert Himports_main]".
+    { transitivity (Some (pc_b ^+ 2)%a); auto; solve_addr. }
+    { solve_addr. }
+    iDestruct (region_pointsto_cons with "Himports_main") as "[Himport_C_f Himports_main]".
+    { transitivity (Some (pc_b ^+ 3)%a); auto; solve_addr. }
+    { solve_addr. }
+
+    (* Revoke the world to get the stack frame *)
+    set ( csp_b := (csp_b' ^+ 4)%a ).
+    set (stk_frame_addrs := finz.seq_between csp_b csp_e).
+    iAssert ([∗ list] a ∈ stk_frame_addrs, ⌜W0.1 !! a = Some Temporary⌝)%I as "Hstk_frm_tmp_W0".
+    { iApply (writeLocalAllowed_valid_cap_implies_full_cap with "Hinterp_W0_csp"); eauto. }
+
+    iMod (monotone_revoke_stack_alt with "[$Hinterp_W0_csp $Hsts_C $Hr_C]")
+        as (l) "(%Hl_unk & Hsts_C & Hr_C & #Hfrm_close_W0 & >[%stk_mem Hstk] & Hrevoked_l)".
+
+    set (W1 := revoke W0).
+    assert (related_sts_priv_world W0 W1) as Hrelated_priv_W0_W1 by eapply revoke_related_sts_priv_world.
+
+
+    (* --------------------------------------------------- *)
+    (* ----------------- Start the proof ----------------- *)
+    (* --------------------------------------------------- *)
+
+    rewrite /so_main_code /SO_main_code_run.
+    rewrite -!app_assoc.
+    rewrite /SO_main_code_f.
+    assert (SubBounds pc_b pc_e (pc_a ^+ length SO_main_code_run)%a
+              (pc_a ^+ length so_main_code)%a).
+    { solve_addr. }
+    focus_block_nochangePC 3 "Hcode_main" as a_f Ha_f "Hcode" "Hcont"; iHide "Hcont" as hcont.
+    replace (pc_b ^+ 23%nat)%a with a_f by solve_addr.
+
+    (* Mov ct1 ca1 *)
+    iInstr "Hcode".
+    subst hcont; unfocus_block "Hcode" "Hcont" as "Hcode_main".
+
+    (* ----------------------------------------------- *)
+    (* ------------- BLOCK 4 : CHECKRA --------------- *)
+    (* ----------------------------------------------- *)
+
+    focus_block 4 "Hcode_main" as a_checkra Ha_checkra "Hcode" "Hcont"; iHide "Hcont" as hcont; clear dependent Ha_f.
+    iApply (checkra_spec with "[- $HPC $Hca0 $Hcs0 $Hcs1 $Hcode]"); eauto.
+    iSplitL; last ( iNext ; iIntros (?); done).
+    iNext ; iIntros "H"; iDestruct "H" as (p g b e a) "(%Hp & HPC & Hca0 & Hcs0 & Hcs1 & Hcode)".
+    subst hcont; unfocus_block "Hcode" "Hcont" as "Hcode_main".
+
+    (* ------------------------------------------------------- *)
+    (* ----------------- BLOCK 5:  CHECKINTS ----------------- *)
+    (* ------------------------------------------------------- *)
+    focus_block 5 "Hcode_main" as a_checkints Ha_checkints "Hcode" "Hcont"; iHide "Hcont" as hcont
+    ; clear dependent Ha_checkra.
+    iAssert (interp )
+    iApply (checkints_spec with "[- $HPC $Hca0 $Hcs0 $Hcs1 $Hcode]"); eauto.
+
+    (* -- separate argument registers -- *)
+    assert ( is_Some (rmap !! ca0) ) as [wca0 Hwca0].
+    { apply Hrmap_init; rewrite Hrmap_dom ; done. }
+    iDestruct (big_sepM_delete _ _ ca0 with "Hrmap") as "[Hca0 Hrmap]"; first by simplify_map_eq.
+    assert ( is_Some (rmap !! ca1) ) as [wca1 Hwca1].
+    { apply Hrmap_init; rewrite Hrmap_dom ; done. }
+    iDestruct (big_sepM_delete _ _ ca1 with "Hrmap") as "[Hca1 Hrmap]"; first by simplify_map_eq.
+    assert ( is_Some (rmap !! ca2) ) as [wca2 Hwca2].
+    { apply Hrmap_init; rewrite Hrmap_dom ; done. }
+    iDestruct (big_sepM_delete _ _ ca2 with "Hrmap") as "[Hca2 Hrmap]"; first by simplify_map_eq.
+    assert ( is_Some (rmap !! ca3) ) as [wca3 Hwca3].
+    { apply Hrmap_init; rewrite Hrmap_dom ; done. }
+    iDestruct (big_sepM_delete _ _ ca3 with "Hrmap") as "[Hca3 Hrmap]"; first by simplify_map_eq.
+    assert ( is_Some (rmap !! ca4) ) as [wca4 Hwca4].
+    { apply Hrmap_init; rewrite Hrmap_dom ; done. }
+    iDestruct (big_sepM_delete _ _ ca4 with "Hrmap") as "[Hca4 Hrmap]"; first by simplify_map_eq.
+    assert ( is_Some (rmap !! ca5) ) as [wca5 Hwca5].
+    { apply Hrmap_init; rewrite Hrmap_dom ; done. }
+    iDestruct (big_sepM_delete _ _ ca5 with "Hrmap") as "[Hca5 Hrmap]"; first by simplify_map_eq.
+
+    focus_block 6 "Hcode_main" as a_call_g1 Ha_call_g1 "Hcode" "Hcont"; iHide "Hcont" as hcont; clear dependent Ha_fetch1.
+    (* Mov cs0 cra *)
+    iInstr "Hcode".
+    (* Mov cs1 ca0 *)
+    iInstr "Hcode".
+    (* Mov ct1 ca0 *)
+    iInstr "Hcode".
+    (* Mov ca0 0 *)
+    iInstr "Hcode".
+    (* Jalr cra ct0 *)
+    iInstr "Hcode".
+
+    set ( rmap_arg :=
+           {[ ca0 := WInt 0;
+              ca1 := wca1;
+              ca2 := wca2;
+              ca3 := wca3;
+              ca4 := wca4;
+              ca5 := wca5;
+              ct0 := WSentry XSRW_ Local b_switcher e_switcher a_switcher_call
+           ]} : Reg
+        ).
+
+    iInsertList "Hrmap" [ct2;ct3].
+    repeat (iEval (rewrite -delete_insert_ne //) in "Hrmap").
+    set (rmap' := (delete ca5 _)).
+    iDestruct (sts_full_rel_loc  with "Hsts_C Hsts_rel") as "%Hwrel_i".
+
+    set (W2 := (<l[i:=false]l>W1)).
+    assert (related_sts_priv_world W1 W2) as Hrelated_priv_W1_W2.
+    { subst W2.
+     rewrite /related_sts_priv_world /=.
+     split; first apply related_sts_std_priv_refl.
+     split;[set_solver|split;[set_solver|] ].
+     intros d rpub rpriv rpub' rpriv' Hr Hr'; simplify_eq.
+     repeat (split; first done).
+     intros x y Hd Hd'.
+     destruct (decide (d = i)); simplify_map_eq; last apply rtc_refl.
+     destruct b; simplify_map_eq; last apply rtc_refl.
+     apply rtc_once.
+     right;apply convert_rel_of_rel.
+     done.
+    }
+
+    assert (related_sts_priv_world W0 W2) as Hrelated_priv_W0_W2 by (by eapply related_sts_priv_trans_world; eauto).
+    assert (related_sts_priv_world W W2) as
+      Hrelated_priv_W_W2 by (by eapply related_sts_priv_trans_world; eauto).
+
+    iMod (update_region_revoked_update_loc with "Hsts_C Hr_C") as "[Hr_C Hsts_C]"; auto.
+    { apply revoke_conditions_sat. }
+
+    (* Show that the arguments are safe, when necessary *)
+    iAssert (if is_sealed_with_o wca0 ot_switcher
+             then (interp W2 C wca0)
+             else True)%I as "#Hinterp_W2_wct1".
+    { destruct (is_sealed_with_o wca0 ot_switcher) eqn:His_sealed_wct1; last done.
+      destruct wca0 as [| [|] | |]; try discriminate.
+      iApply (interp_monotone_sd W0 W2); eauto.
+      iApply "Hinterp_rmap"; eauto.
+      iPureIntro ; set_solver.
+    }
+    iAssert ( ⌜ wca1 = WInt 0 ⌝ )%I as "->".
+    { iApply "Hzeroed_rmap"; eauto.
+      set_solver+.
+    }
+    iAssert ( ⌜ wca2 = WInt 0 ⌝ )%I as "->".
+    { iApply "Hzeroed_rmap"; eauto.
+      set_solver+.
+    }
+    iAssert ( ⌜ wca3 = WInt 0 ⌝ )%I as "->".
+    { iApply "Hzeroed_rmap"; eauto.
+      set_solver+.
+    }
+    iAssert ( ⌜ wca4 = WInt 0 ⌝ )%I as "->".
+    { iApply "Hzeroed_rmap"; eauto.
+      set_solver+.
+    }
+    iAssert ( ⌜ wca5 = WInt 0 ⌝ )%I as "->".
+    { iApply "Hzeroed_rmap"; eauto.
+      set_solver+.
+    }
+
+    iAssert ([∗ map] rarg↦warg ∈ rmap_arg , rarg ↦ᵣ warg ∗ interp W2 C warg)%I
+      with "[Hca0 Hca1 Hca2 Hca3 Hca4 Hca5 Hct0]" as "Hrmap_arg".
+    { subst rmap_arg.
+      iAssert (interp W2 C (WInt 0)) as "Hinterp_0"; first iApply interp_int.
+      iAssert (interp W2 C (WSentry XSRW_ Local b_switcher e_switcher a_switcher_call)) as
+        "Hinterp_sw_call"; first iApply interp_switcher_call; auto.
+      repeat (iApply big_sepM_insert; [done|iFrame "∗#"]).
+      done.
+    }
+
+    (* Prepare the closing resources for the switcher call spec *)
+    iAssert (
+        ([∗ list] a ∈ finz.seq_between csp_b csp_e, closing_revoked_resources W2 C a ∗
+                                                    ⌜W2.1 !! a = Some Revoked⌝)
+      )%I with "[Hfrm_close_W0]" as "Hfrm_close_W2".
+    {
+      iApply (big_sepL_impl with "Hfrm_close_W0").
+      iModIntro; iIntros (k a Ha) "[Hclose %Hrev]".
+      iDestruct (mono_priv_closing_revoked_resources with "Hclose") as "$"; auto.
+    }
+    subst hcont; unfocus_block "Hcode" "Hcont" as "Hcode_main".
+
+    iMod ("Hvae_code_close" with "[$Hna Himport_assert Himport_switcher Himport_C_f Himports_main $Hcode_main]")
+      as "Hna".
+    { iNext.
+      iDestruct (region_pointsto_cons with "[$Himport_C_f $Himports_main]") as "Himports_main"
+      ; [solve_addr|solve_addr|].
+      iDestruct (region_pointsto_cons with "[$Himport_assert $Himports_main]") as "Himports_main"
+      ; [solve_addr|solve_addr|].
+      iDestruct (region_pointsto_cons with "[$Himport_switcher $Himports_main]") as "$" ;solve_addr.
+    }
+
+    (* Apply the spec switcher call *)
+    iApply (switcher_cc_specification_alt with
+             "[- $Hswitcher $Hna
+              $HPC $Hcgp $Hcra $Hcsp $Hct1 $Hcs0 $Hcs1 $Hrmap_arg $Hrmap
+              $Hstk $Hr_C $Hsts_C $Hfrm_close_W2 $Hcstk
+              $Hinterp_W2_wct1 $HK]"); eauto.
+    { subst rmap'.
+      repeat (rewrite dom_delete_L); repeat (rewrite dom_insert_L).
+      apply regmap_full_dom in Hrmap_init.
+      rewrite /dom_arg_rmap Hrmap_init.
+      set_solver+.
+    }
+    { by rewrite /is_arg_rmap. }
+
+    iClear "Hinterp_rmap Hzeroed_rmap".
+    clear dependent wct1 wct0 wct2 wct3 wcs0 wcs1 rmap stk_mem.
+    iNext.
+    iIntros (W3 rmap stk_mem l')
+      "( _ & _ & %Hrelated_pub_2ext_W3 & Hrel_stk_C' & %Hdom_rmap & Hfrm_close_W3
+      & Hna & %Hcsp_bounds
+      & Hsts_C & Hr_C
+      & Hcstk_frag
+      & HPC & Hcgp & Hcra & Hcs0 & Hcs1 & Hcsp
+      & [%warg0 [Hca0 _] ] & [%warg1 [Hca1 _] ]
+      & Hrmap & Hstk & HK)"; clear l'.
+    iEval (cbn) in "HPC".
+
+    assert (related_sts_pub_world W2 W3) as Hrelated_pub_W2_W3.
+    {
+      eapply related_sts_pub_trans_world ; eauto.
+      apply related_sts_pub_update_multiple_temp.
+      apply Forall_forall; intros a Ha.
+      cbn.
+      eapply revoke_lookup_Monotemp.
+      destruct Hl_unk as [_ Htemp]; apply Htemp.
+      apply elem_of_app; right.
+      rewrite !elem_of_finz_seq_between in Ha |- *; solve_addr+Ha.
+    }
+    set (W4 := revoke W3).
+
+    (* simplify the knowledge about the new rmap *)
+    iDestruct (big_sepM_sep with "Hrmap") as "[Hrmap Hrmap_zero]".
+    iDestruct (big_sepM_pure with "Hrmap_zero") as "%Hrmap_zero".
+    assert (∀ r : RegName, r ∈ dom rmap → rmap !! r = Some (WInt 0)) as Hrmap_init.
+    { intros r Hr.
+      rewrite elem_of_dom in Hr. destruct Hr as [wr Hr].
+      pose proof Hr as Hr'.
+      eapply map_Forall_lookup in Hr'; eauto.
+      by cbn in Hr' ; simplify_eq.
+    }
+    iClear "Hrmap_zero".
+
+    (* ---- extract the needed registers ct0 ct1 ----  *)
+    iExtractList "Hrmap" [ct0;ct1] as ["Hct0"; "Hct1"].
+
+    iMod (na_inv_acc with "Hvae_code Hna")
+      as "(( >Himports_main & >Hcode_main) & Hna & Hvae_code_close)"; auto.
+    clear Hpc_contiguous.
+    codefrag_facts "Hcode_main" ; rename H into Hpc_contiguous; clear H0.
+
+    (* Extract the imports *)
+    iDestruct (region_pointsto_cons with "Himports_main") as "[Himport_switcher Himports_main]".
+    { transitivity (Some (pc_b ^+ 1)%a); auto; solve_addr. }
+    { solve_addr. }
+
+    clear a_awkward.
+    focus_block_nochangePC 7 "Hcode_main" as a_awkward Ha_awkward "Hcode" "Hcont"; iHide "Hcont" as hcont.
+    replace (a_call_g1 ^+ 5)%a with a_awkward by solve_addr.
+
+    (* Store cgp 1%Z; *)
+    iInstr_lookup "Hcode" as "Hi" "Hcode".
+    wp_instr.
+    iMod (inv_acc with "HawkN") as "(>(%b' & Hst_i & Hcgp_b) & Hclose_awk)"; auto.
+    iAssert ( cgp_b ↦ₐ (if b' then WInt 1 else WInt 0) )%I with "[Hcgp_b]" as "Hcgp_b".
+    { destruct b' ; iFrame. }
+    iApply (wp_store_success_z with "[$HPC $Hi $Hcgp $Hcgp_b]"); try solve_pure.
+    { apply withinBounds_true_iff; solve_addr. }
+    iIntros "!> (HPC & Hi & Hcgp & Hcgp_b)".
+    iDestruct (sts_full_state_loc  with "Hsts_C Hst_i") as "%Hwst_i'".
+    iMod (sts_update_loc _ _ _ _ true with "Hsts_C Hst_i") as "[Hsts_C Hst_i]".
+    iMod ("Hclose_awk" with "[$Hst_i $Hcgp_b]") as "_".
+    iModIntro.
+    wp_pure.
+    iSpecialize ("Hcode" with "[$]").
+
+    (* Mov cra cs0 *)
+    iInstr "Hcode".
+    (* Mov ct1 cs1 *)
+    iInstr "Hcode".
+    subst hcont; unfocus_block "Hcode" "Hcont" as "Hcode_main".
+
+    (* --------------------------------------------------- *)
+    (* ---------------- BLOCK 9 : FETCH ------------------ *)
+    (* --------------------------------------------------- *)
+
+    focus_block 8 "Hcode_main" as a_fetch2 Ha_fetch2 "Hcode" "Hcont"; iHide "Hcont" as hcont; clear dependent Ha_awkward.
+    iApply (fetch_spec with "[- $HPC $Hct0 $Hcs0 $Hcs1 $Hcode]"); eauto.
+    { apply withinBounds_true_iff; solve_addr. }
+    replace (pc_b ^+ 0)%a with pc_b by solve_addr.
+    iFrame "Himport_switcher".
+    iNext ; iIntros "(HPC & Hct0 & Hcs0 & Hcs1 & Hcode & Himport_switcher)".
+    iEval (cbn) in "Hct0".
+    subst hcont; unfocus_block "Hcode" "Hcont" as "Hcode_main".
+
+    focus_block 9 "Hcode_main" as a_call_g2 Ha_call_g2 "Hcode" "Hcont"; iHide "Hcont" as hcont
+    ; clear dependent Ha_fetch2.
+    (* Mov cs0 cra *)
+    iInstr "Hcode".
+    (* Mov ca0 0 *)
+    iInstr "Hcode".
+    (* Mov ca1 0 *)
+    iInstr "Hcode".
+    (* Jalr cra ct0 *)
+    iInstr "Hcode".
+
+    (* -- separate argument registers -- *)
+    assert ( rmap !! ca2 = Some (WInt 0)) as Hwca2.
+    { apply Hrmap_init; rewrite Hdom_rmap; set_solver+. }
+    assert ( rmap !! ca3 = Some (WInt 0)) as Hwca3.
+    { apply Hrmap_init; rewrite Hdom_rmap; set_solver+. }
+    assert ( rmap !! ca4 = Some (WInt 0)) as Hwca4.
+    { apply Hrmap_init; rewrite Hdom_rmap; set_solver+. }
+    assert ( rmap !! ca5 = Some (WInt 0)) as Hwca5.
+    { apply Hrmap_init; rewrite Hdom_rmap; set_solver+. }
+    iExtractList "Hrmap" [ca2;ca3;ca4;ca5] as ["Hca2"; "Hca3"; "Hca4"; "Hca5"].
+
+    clear rmap_arg.
+    set ( rmap_arg :=
+           {[ ca0 := WInt 0;
+              ca1 := WInt 0;
+              ca2 := WInt 0;
+              ca3 := WInt 0;
+              ca4 := WInt 0;
+              ca5 := WInt 0;
+              ct0 := WSentry XSRW_ Local b_switcher e_switcher a_switcher_call
+           ]} : Reg
+        ).
+    set (rmap' := (delete ca5 _)).
+
+
+    iDestruct (sts_full_rel_loc  with "Hsts_C Hsts_rel") as "%Hwrel_i'".
+    set (W5 := (<l[i:=true]l>W4)).
+    assert (related_sts_pub_world W4 W5) as Hpriv_W4_W5.
+    { subst W5.
+     rewrite /related_sts_pub_world /=.
+     split; first apply related_sts_std_pub_refl.
+     split;[set_solver|split;[set_solver|] ].
+     intros d rpub rpriv rpub' rpriv' Hr Hr'; simplify_eq.
+     repeat (split; first done).
+     intros x y Hd Hd'.
+     destruct (decide (d = i)); simplify_map_eq; last apply rtc_refl.
+     destruct b'; simplify_map_eq; first apply rtc_refl.
+     apply rtc_once.
+     rewrite /convert_rel.
+     exists false, true.
+     repeat (split; first done).
+     by rewrite /awk_rel_pub; left.
+    }
+
+    assert (related_sts_priv_world W3 W5) as Hrelated_priv_W3_W5.
+    { eapply (related_sts_priv_pub_trans_world W3 W4); eauto.
+      apply revoke_related_sts_priv_world.
+    }
+    assert (related_sts_priv_world W2 W5) as Hrelated_priv_W2_W5.
+    { eapply related_sts_pub_priv_trans_world; eauto. }
+
+    iMod (update_region_revoked_update_loc with "Hsts_C Hr_C") as "[Hr_C Hsts_C]"; auto.
+    { apply revoke_conditions_sat. }
+    { by apply related_sts_pub_priv_world. }
+
+    (* Show that the arguments are safe, when necessary *)
+    iAssert ([∗ map] rarg↦warg ∈ rmap_arg , rarg ↦ᵣ warg ∗ interp W5 C warg)%I
+      with "[Hca0 Hca1 Hca2 Hca3 Hca4 Hca5 Hct0]" as "Hrmap_arg".
+    { subst rmap_arg.
+      iAssert (interp W5 C (WInt 0)) as "Hinterp_0"; first iApply interp_int.
+      iAssert (interp W5 C (WSentry XSRW_ Local b_switcher e_switcher a_switcher_call)) as
+        "Hinterp_sw_call"; first iApply interp_switcher_call; auto.
+      repeat (iApply big_sepM_insert; [done|iFrame "∗#"]).
+      done.
+    }
+
+    (* Show that the arguments are safe, when necessary *)
+    iAssert (if is_sealed_with_o wca0 ot_switcher
+             then (interp W5 C wca0)
+             else True)%I as "#Hinterp_W5_wca0".
+    { destruct (is_sealed_with_o wca0 ot_switcher) eqn:His_sealed_wca0; last done.
+      destruct wca0 as [| [|] | |]; try discriminate.
+      iApply (interp_monotone_sd W2 W5); eauto.
+    }
+
+    (* Prepare the closing resources for the switcher call spec *)
+    iAssert (
+        ([∗ list] a ∈ finz.seq_between csp_b csp_e, closing_revoked_resources W5 C a ∗
+                                                    ⌜W5.1 !! a = Some Revoked⌝)
+      )%I with "[Hfrm_close_W3]" as "#Hfrm_close_W5".
+    { rewrite !big_sepL_sep.
+      iDestruct "Hfrm_close_W3" as "[Hclose_W3 %Hrev_W3]".
+      iSplitL "Hclose_W3".
+      - iApply (big_sepL_impl with "Hclose_W3").
+        iModIntro; iIntros (k a Ha) "Hclose'".
+        iApply mono_priv_closing_revoked_resources; last done.
+        eauto.
+      - iApply big_sepL_pure; iPureIntro.
+        intros k x Hk.
+        cbn.
+        eapply Hrev_W3; eauto.
+    }
+    subst hcont; unfocus_block "Hcode" "Hcont" as "Hcode_main".
+
+    iMod ("Hvae_code_close" with "[$Hna Himport_switcher Himports_main $Hcode_main]")
+      as "Hna".
+    { iNext.
+      iDestruct (region_pointsto_cons with "[$Himport_switcher $Himports_main]") as "$" ;solve_addr.
+    }
+
+    iDestruct (sts_full_rel_loc  with "Hsts_C Hsts_rel") as "%Hwrel_i_W5".
+    (* Apply the spec switcher call *)
+    iApply (switcher_cc_specification_alt with
+             "[- $Hswitcher $Hna
+              $HPC $Hcgp $Hcra $Hcsp $Hct1 $Hcs0 $Hcs1 $Hrmap_arg $Hrmap
+              $Hstk $Hr_C $Hsts_C $Hfrm_close_W5 $Hcstk_frag
+              $Hinterp_W5_wca0 $HK]"); eauto.
+    { subst rmap'.
+      repeat (rewrite dom_delete_L); repeat (rewrite dom_insert_L).
+      rewrite Hdom_rmap.
+      set_solver+.
+    }
+    { by rewrite /is_arg_rmap. }
+
+    clear dependent wct1 wct0 warg0 warg1 rmap stk_mem Hcsp_bounds.
+    iNext.
+    iIntros (W6 rmap stk_mem l')
+      "(_ & _ & %Hrelated_pub_5ext_W6 & Hrel_stk_C'' & %Hdom_rmap & Hfrm_close_W6
+      & Hna & %Hcsp_bounds
+      & Hsts_C & Hr_C
+      & Hcstk_frag
+      & HPC & Hcgp & Hcra & Hcs0 & Hcs1 & Hcsp
+      & [%warg0 [Hca0 _] ] & [%warg1 [Hca1 _] ]
+      & Hrmap & Hstk & HK)"; clear l'.
+    iEval (cbn) in "HPC".
+
+    (* Derive some information necessary later *)
+    iAssert ( ⌜ Forall (λ k : finz MemNum, W5.1 !! k = Some Revoked) (finz.seq_between (csp_b ^+ 4)%a csp_e) ⌝)%I
+      as "%Hrevoked_stk_W5".
+    { iClear "∗".
+      iDestruct (big_sepL_sep with "Hfrm_close_W5") as "[_ %]".
+      iPureIntro.
+      apply Forall_forall.
+      intros x Hx.
+      assert (x ∈ finz.seq_between csp_b csp_e) as Hx'.
+      {
+        rewrite (finz_seq_between_split csp_b (csp_b ^+ 4)%a csp_e); last solve_addr.
+        rewrite elem_of_app; by right.
+      }
+      apply elem_of_list_lookup in Hx' as [k Hk].
+      eapply H; eauto.
+    }
+    assert (related_sts_pub_world W5 W6) as Hrelated_pub_W5_W6.
+    { clear -Hrelated_pub_5ext_W6 Hrevoked_stk_W5.
+      eapply related_sts_pub_trans_world; eauto.
+      eapply related_sts_pub_update_multiple_temp; eauto.
+    }
+    clear Hrevoked_stk_W5.
+
+    iAssert (⌜ Forall (λ a : finz MemNum, a ∈ dom W6.1) l ⌝)%I as "%Hl_revoked_W6".
+    {
+      iDestruct (big_sepL_sep with "Hrevoked_l") as "[_ %Hrevoked_l]".
+      iPureIntro; apply Forall_forall; intros a Ha.
+      apply elem_of_list_lookup in Ha as [k Hk].
+      apply Hrevoked_l in Hk.
+      cbn.
+      assert (a ∈ dom (std W2)) as Ha2.
+      { rewrite elem_of_dom; done. }
+      destruct Hrelated_pub_W5_W6 as [ [Hdom_5_6 _] _ ].
+      apply Hdom_5_6.
+      cbn.
+      rewrite -revoke_dom_eq.
+      destruct Hrelated_pub_W2_W3 as [ [Hdom_2_3 _] _ ].
+      by apply Hdom_2_3.
+    }
+
+    set (W7 := revoke W6).
+    iMod (
+       revoked_by_separation_many_with_temp_resources with "[$Hsts_C $Hr_C $Hrevoked_l]"
+      ) as "(Hrevoked_l & Hsts_C & Hr_C & %Hl_revoked_W7)".
+    { apply Forall_forall; intros a Ha.
+      rewrite Forall_forall in Hl_revoked_W6.
+      apply Hl_revoked_W6 in Ha.
+      rewrite -revoke_dom_eq.
+      done.
+    }
+
+
+    (* simplify the knowledge about the new rmap *)
+    iDestruct (big_sepM_sep with "Hrmap") as "[Hrmap Hrmap_zero]".
+    iDestruct (big_sepM_pure with "Hrmap_zero") as "%Hrmap_zero".
+    assert (∀ r : RegName, r ∈ dom rmap → rmap !! r = Some (WInt 0)) as Hrmap_init.
+    { intros r Hr.
+      rewrite elem_of_dom in Hr. destruct Hr as [wr Hr].
+      pose proof Hr as Hr'.
+      eapply map_Forall_lookup in Hr'; eauto.
+      by cbn in Hr' ; simplify_eq.
+    }
+    iClear "Hrmap_zero".
+
+    (* ---- extract the needed registers ct0 ct1 ----  *)
+    iExtractList "Hrmap" [ct0;ct1] as ["Hct0"; "Hct1"].
+
+    iMod (na_inv_acc with "Hvae_code Hna")
+      as "(( >Himports_main & >Hcode_main) & Hna & Hvae_code_close)"; auto.
+    clear Hpc_contiguous.
+    codefrag_facts "Hcode_main" ; rename H into Hpc_contiguous; clear H0.
+
+    (* Extract the imports *)
+    iDestruct (region_pointsto_cons with "Himports_main") as "[Himport_switcher Himports_main]".
+    { transitivity (Some (pc_b ^+ 1)%a); auto; solve_addr. }
+    { solve_addr. }
+    iDestruct (region_pointsto_cons with "Himports_main") as "[Himport_assert Himports_main]".
+    { transitivity (Some (pc_b ^+ 2)%a); auto; solve_addr. }
+    { solve_addr. }
+
+    clear a_awkward.
+    focus_block_nochangePC 9 "Hcode_main" as a_ret Ha_ret "Hcode" "Hcont"; iHide "Hcont" as hcont.
+    replace a_call_g2 with a_ret by solve_addr.
+
+    iInstr_lookup "Hcode" as "Hi" "Hcode".
+    wp_instr.
+    iMod (inv_acc with "HawkN") as "(>(%b'' & Hst_i & Hcgp_b) & Hclose_awk)"; auto.
+    iDestruct (sts_full_state_loc  with "Hsts_C Hst_i") as "%Hwst_i''".
+    iDestruct (sts_full_rel_loc  with "Hsts_C Hsts_rel") as "%Hwrel_i''".
+    assert (loc W7 !! i = Some (encode true)); last simplify_eq.
+    {
+      destruct Hrelated_pub_W5_W6 as [_ [Hdom1 [Hdom2 Htrans] ] ].
+      specialize (Htrans i _ _ _ _ Hwrel_i_W5 Hwrel_i'') as [Heq1 [Heq2 Htrans] ]; eauto .
+      assert (loc W5 !! i = Some (encode true)) by (by simplify_map_eq).
+      specialize (Htrans _ _ H2 Hwst_i'').
+      apply rtc_rel_pub' in Htrans ; auto.
+      simplify_eq; auto.
+    }
+
+    iApply (wp_load_success_alt with "[$HPC $Hi $Hct0 $Hcgp $Hcgp_b]"); try solve_pure.
+    { split; last apply withinBounds_true_iff; solve_addr. }
+    iIntros "!> (HPC & Hct0 & Hi & Hcgp & Hcgp_b)".
+    iMod ("Hclose_awk" with "[$Hst_i $Hcgp_b]") as "_".
+    iModIntro.
+    wp_pure.
+    iSpecialize ("Hcode" with "[$]").
+    iEval (cbn) in "Hct0".
+
+    (* Mov ct1 1%Z; *)
+    iInstr "Hcode".
+
+    subst hcont; unfocus_block "Hcode" "Hcont" as "Hcode_main".
+
+    (* --------------------------------------------------- *)
+    (* ----------------- BLOCK 4: ASSERT ----------------- *)
+    (* --------------------------------------------------- *)
+
+    focus_block 10 "Hcode_main" as a_assert_c Ha_assert_c "Hcode" "Hcont"; iHide "Hcont" as hcont.
+    iExtractList "Hrmap" [ct2;ct3;ct4] as ["Hct2"; "Hct3";"Hct4"].
+    iApply (assert_success_spec
+             with
+             "[- $Hassert $Hna $HPC $Hct2 $Hct3 $Hct4 $Hct0 $Hct1 $Hcra
+              $Hcode $Himport_assert]") ; auto.
+    { apply withinBounds_true_iff; solve_addr. }
+    { solve_ndisj. }
+    iNext; iIntros "(Hna & HPC & Hct2 & Hct3 & Hct4 & Hcra & Hct0 & Hct1
+                    & Hcode & Himport_assert)".
+    subst hcont; unfocus_block "Hcode" "Hcont" as "Hcode_main".
+
+    (* --------------------------------------------------- *)
+    (* ----------------- BLOCK 5: RETURN ----------------- *)
+    (* --------------------------------------------------- *)
+    focus_block 11 "Hcode_main" as a_halt Ha_halt "Hcode" "Hcont"; iHide "Hcont" as hcont.
+    (* Mov cra cs0; *)
+    iInstr "Hcode".
+    (* Mov ca0 0%Z; *)
+    iInstr "Hcode".
+    (* Mov ca1 0%Z; *)
+    iInstr "Hcode".
+    (* JmpCap cra *)
+    iInstr "Hcode".
+    subst hcont; unfocus_block "Hcode" "Hcont" as "Hcode_main".
+
+    iMod ("Hvae_code_close" with "[$Hna Himport_switcher Himport_assert Himports_main $Hcode_main]")
+      as "Hna".
+    { iNext.
+      iDestruct (region_pointsto_cons with "[$Himport_assert $Himports_main]") as "Himports_main"
+      ; [solve_addr|solve_addr|].
+      iDestruct (region_pointsto_cons with "[$Himport_switcher $Himports_main]") as "$" ;solve_addr.
+    }
+
+    (* Put all the registers under the same map *)
+    iInsertList "Hrmap" [ct4;ct3;ct2;ct1;ct0].
+    iDestruct (big_sepM_insert _ _ cs0 with "[$Hrmap $Hcs0]") as "Hrmap".
+    { repeat (rewrite lookup_insert_ne; auto); apply not_elem_of_dom_1; rewrite Hdom_rmap; set_solver+. }
+    iDestruct (big_sepM_insert _ _ cs1 with "[$Hrmap $Hcs1]") as "Hrmap".
+    { repeat (rewrite lookup_insert_ne; auto); apply not_elem_of_dom_1; rewrite Hdom_rmap; set_solver+. }
+    iDestruct (big_sepM_insert _ _ cgp with "[$Hrmap $Hcgp]") as "Hrmap".
+    { repeat (rewrite lookup_insert_ne; auto); apply not_elem_of_dom_1; rewrite Hdom_rmap; set_solver+. }
+    iDestruct (big_sepM_insert _ _ cra with "[$Hrmap $Hcra]") as "Hrmap".
+    { repeat (rewrite lookup_insert_ne; auto); apply not_elem_of_dom_1; rewrite Hdom_rmap; set_solver+. }
+
+    iDestruct (big_sepL_sep with "Hfrm_close_W6") as "[_ %Hrevoked_stk_W7]".
+    iApply (switcher_ret_specification _ W0 W7
+             with
+             "[ $Hswitcher $Hstk $Hcstk_frag $HK $Hsts_C $Hna $HPC $Hr_C $Hrevoked_l
+             $Hrmap $Hca0 $Hca1 $Hcsp]"
+           ); auto.
+    { destruct Hl_unk as [_ ?].
+      eapply (related_pub_W0_Wfixed W0 W3 W6 l); eauto.
+      apply Forall_app; split; auto.
+      apply Forall_forall; intros a Ha.
+      apply elem_of_list_lookup in Ha ; destruct Ha as [??]; eapply Hrevoked_stk_W7; eauto.
+    }
+    { repeat (rewrite dom_insert_L); rewrite Hdom_rmap; set_solver+. }
+    { subst csp_b.
+      destruct Hsync_csp as [].
+      rewrite -H0; auto.
+    }
+    { destruct Hl_unk; auto. }
+    { destruct Hl_unk; auto. }
+    { iSplit; iApply interp_int. }
+  Qed.
+
+  Lemma vae_awkward_safe
+
+    (pc_b pc_e pc_a : Addr)
+    (cgp_b cgp_e : Addr)
+
+    (b_vae_exp_tbl e_vae_exp_tbl : Addr)
+
+    (b_assert e_assert : Addr) (a_flag : Addr)
+    (C_f : Sealable)
+
+    (W : WORLD)
+
+    (Nassert Nswitcher Nvae VAEN : namespace)
+    i
+
+    :
+
+    let imports :=
+     vae_main_imports
+       b_switcher e_switcher a_switcher_call ot_switcher b_assert e_assert C_f
+    in
+
+    Nswitcher ## Nassert ->
+    Nswitcher ## Nvae ->
+    Nassert ## Nvae ->
+    (b_vae_exp_tbl <= b_vae_exp_tbl ^+ 2 < e_vae_exp_tbl)%a ->
+    SubBounds pc_b pc_e pc_a (pc_a ^+ length (vae_main_code ot_switcher))%a ->
+    (pc_b + length imports)%a = Some pc_a ->
+    (cgp_b + length vae_main_data)%a = Some cgp_e ->
+    (exists b : bool, loc W !! i = Some (encode b)) ->
+    wrel W !! i =
+    Some (convert_rel awk_rel_pub, convert_rel awk_rel_priv) ->
+
+    na_inv logrel_nais Nassert (assert_inv b_assert e_assert a_flag)
+    ∗ na_inv logrel_nais Nswitcher switcher_inv
+    ∗ na_inv logrel_nais Nvae
+        ([[ pc_b , pc_a ]] ↦ₐ [[ imports ]] ∗ codefrag pc_a (vae_main_code ot_switcher))
+    ∗ inv (export_table_PCCN VAEN) (b_vae_exp_tbl ↦ₐ WCap RX Global pc_b pc_e pc_b)
+    ∗ inv (export_table_CGPN VAEN) ((b_vae_exp_tbl ^+ 1)%a ↦ₐ WCap RW Global cgp_b cgp_e cgp_b)
+    ∗ inv (export_table_entryN VAEN (b_vae_exp_tbl ^+ 2)%a)
+        ((b_vae_exp_tbl ^+ 2)%a ↦ₐ WInt (encode_entry_point 1 (length (imports ++ VAE_main_code_init))))
+    ∗ WSealed ot_switcher (SCap RO Global b_vae_exp_tbl e_vae_exp_tbl (b_vae_exp_tbl ^+ 2)%a)
+        ↦□ₑ 1
+    ∗ WSealed ot_switcher (SCap RO Local b_vae_exp_tbl e_vae_exp_tbl (b_vae_exp_tbl ^+ 2)%a)
+        ↦□ₑ 1
+    ∗ seal_pred ot_switcher ot_switcher_propC
+    ∗ (∃ ι, inv ι (awk_inv C i cgp_b))
+    ∗ sts_rel_loc (A:=Addr) C i awk_rel_pub awk_rel_priv
+      -∗
+    interp W C
+      (WSealed ot_switcher (SCap RO Global b_vae_exp_tbl e_vae_exp_tbl (b_vae_exp_tbl ^+ 2)%a)).
+  Proof.
+    intros imports; subst imports.
+    iIntros (Hswitcher_assert HNswitcher_vae HNassert_vae
+               Hvae_exp_tbl_size Hvae_size_code Hvae_imports Hcgp_size Hloc_i_W Hrel_i_W)
+      "(#Hassert & #Hswitcher
+      & #Hvae_code
+      & #Hvae_exp_PCC
+      & #Hvae_exp_CGP
+      & #Hvae_exp_awkward
+      & #Hentry_VAE & #Hentry_VAE' & #Hot_switcher
+      & [%ι #Hι] & #Hsts_rel)".
+    iEval (rewrite fixpoint_interp1_eq /=).
+    rewrite /interp_sb.
+    iFrame "Hot_switcher".
+    iSplit; [iPureIntro; apply persistent_cond_ot_switcher |].
+    iSplit; [iIntros (w); iApply mono_priv_ot_switcher|].
+    iSplit; iNext ; iApply vae_awkward_spec; try iFrame "#"; eauto.
+  Qed.
+
+
+End VAE.
